wip with Vimala

ictr_new.fst
@@ -18,7 +18,7 @@ type log_entry = timestamp_t & op_t
 type log = seq log_entry
 
 unfold
-  let ( ++ ) (l1 l2:log) = Seq.append l1 l2
+let ( ++ ) (l1 l2:log) = Seq.append l1 l2
 
 let distinct_ops (l:log) : prop = forall (e:log_entry). count e l <= 1
 
@@ -42,7 +42,7 @@ let rec seq_foldl (f:concrete_st -> log_entry -> concrete_st) (x:concrete_st) (s
             seq_foldl f (f x hd) tl
 
 // apply an operation to a state
-let do (s:concrete_st) (o:log_entry) : (r:concrete_st{r = s + 1}) = s + 1
+let do (s:concrete_st) (_:log_entry) : concrete_st = s + 1
 
 let valid_st (s:st0) : prop =
   (*)distinct_ops (ops_of s) /\*)
@@ -56,9 +56,13 @@ let rec lem_foldl (s:concrete_st) (l:log)
     |0 -> ()
     |_ -> lem_foldl (do s (head l)) (tail l)
 
-let linearized_merge (s:concrete_st) (l:log) : (r:st{v_of r = seq_foldl do s l}) =
-  let r = (seq_foldl do s l, hide (s,l)) in
-  lem_foldl s l; r
+let st_inv (s:st)
+  : Lemma (v_of s == init_of s + Seq.length (snd (snd s))) = admit ()
+
+let linearized_merge (s:concrete_st) (l:log) : st = seq_foldl do s l, hide (s,l)
+
+let linearized_merge_spec (s:concrete_st) (l:log)
+  : Lemma (v_of (linearized_merge s l) == s + Seq.length l) = admit ()
 
 //conflict resolution
 let resolve_conflict (x y:log_entry) : log =
@@ -82,53 +86,79 @@ let resolve_conflict_mem (x y:log_entry)
            (Seq.length s == 2 ==> is_x_and_y s x y))
   = ()
 
+irreducible let pat (l:log) : unit = ()
 
 #set-options "--query_stats"
 // l is interleaving of l1 and l2
 let rec is_interleaving (l l1 l2:log) 
   : Tot Type0 (decreases %[Seq.length l1; Seq.length l2]) =
 
-  // l1 and l2 are empty
-    ((Seq.length l1 == 0 /\ Seq.length l2 == 0) ==> l == empty) 
+  // // l1 and l2 are empty
+  //   ((Seq.length l1 == 0 /\ Seq.length l2 == 0) ==> l == empty) 
 
-    /\
+  //   /\
 
   // if l1 is empty, then l == l2
-  (Seq.length l1 == 0 /\ Seq.length l2 <> 0 ==> l == l2)
+  (Seq.length l1 == 0 ==> l == l2)
 
   /\
 
   // similarly for l2 being empty
-  (Seq.length l2 == 0 /\ Seq.length l1 <> 0 ==> l == l1)
+  (Seq.length l2 == 0 ==> l == l1)
 
   /\
 
-  // length of l1 and l2 = 1
-  ((Seq.length l1 = 1 /\ Seq.length l2 = 1) ==>
+  // // length of l1 and l2 = 1
+  // ((Seq.length l1 = 1 /\ Seq.length l2 = 1) ==>
 
-    l == (resolve_conflict (last l1) (last l2)))
+  //   l == (resolve_conflict (last l1) (last l2)))
 
-  /\
+  // /\
 
   // if both are non-empty and lengths > 1
   // then three cases
-  ((Seq.length l1 > 1 /\ Seq.length l2 > 1) ==>
+  ((Seq.length l1 > 0 /\ Seq.length l2 > 0) ==>
 
    (let prefix1, last1 = un_snoc l1 in
     let prefix2, last2 = un_snoc l2 in
 
-    (exists l'. is_interleaving l' prefix1 prefix2 /\
-           l == l' ++ (resolve_conflict last1 last2))
+    (exists l'.
+          is_interleaving l' prefix1 prefix2 /\
+          l == l' ++ (resolve_conflict last1 last2))
 
     \/
 
-    (exists l'. is_interleaving l' l1 prefix2 /\
-           l == Seq.snoc l' last2)
+    (exists l'.
+          is_interleaving l' l1 prefix2 /\
+          l == Seq.snoc l' last2)
 
     \/
 
-    (exists l'. is_interleaving l' prefix1 l2 /\
-           l == Seq.snoc l' last1)))
+    (exists l'.
+          is_interleaving l' prefix1 l2 /\
+          l == Seq.snoc l' last1)))
+
+let interleaving_helper (l1 l2 l':log)
+  : Lemma
+      (requires
+         Seq.length l1 > 0 /\ Seq.length l2 > 0 /\
+         (let prefix1, last1 = un_snoc l1 in
+          let prefix2, last2 = un_snoc l2 in
+          is_interleaving l' prefix1 prefix2))
+      (ensures 
+         (let prefix1, last1 = un_snoc l1 in
+          let prefix2, last2 = un_snoc l2 in
+          is_interleaving (Seq.append l' (resolve_conflict last1 last2)) l1 l2))
+  = let prefix1, last1 = un_snoc l1 in
+    let prefix2, last2 = un_snoc l2 in
+    let l = Seq.append l' (resolve_conflict last1 last2) in
+    introduce exists l'. is_interleaving l' prefix1 prefix2 /\
+                    l == Seq.append l' (resolve_conflict last1 last2)
+    with l'
+    and ()
+
+         
+              
 
 // concrete merge pre-condition
 let concrete_merge_pre (lca a b:concrete_st) : prop
@@ -138,17 +168,17 @@ let concrete_merge_pre (lca a b:concrete_st) : prop
 let concrete_merge (lca:concrete_st) (cst1:concrete_st) (cst2:concrete_st{concrete_merge_pre lca cst1 cst2}) 
   : concrete_st = cst1 + cst2 - lca
 
-let inverse (s:st{length (ops_of s) <> 0}) 
-          : GTot (r:concrete_st{let p, l = un_snoc (ops_of s) in
-                      (r == seq_foldl do (init_of s) p)})
+let inverse (s:st{length (ops_of s) > 0}) : GTot concrete_st
+          // : GTot (r:concrete_st{let p, l = un_snoc (ops_of s) in
+          //             (r == seq_foldl do (init_of s) p)})
     = let p, l = un_snoc (ops_of s) in
       let r = seq_foldl do (init_of s) p in
       r
 
 let rec lem_inverse (s:st)
-  : Lemma (requires length (ops_of s) <> 0)
+  : Lemma (requires length (ops_of s) > 0)
           (ensures (v_of s == do (inverse s) (last (ops_of s))) /\
-                   (inverse s >= init_of s) /\ (v_of s = init_of s + length (ops_of s)) /\ (v_of s >= init_of s))
+                   (inverse s >= init_of s) /\ (v_of s = init_of s + length (ops_of s)))
           (decreases length (ops_of s))
   = match length (ops_of s) with
     |0 -> ()
@@ -157,22 +187,31 @@ let rec lem_inverse (s:st)
                      (hide (do (init_of s) (head (ops_of s)), (tail (ops_of s)))))
 
 
+let inverse_st (s:st{Seq.length (ops_of s) > 0}) : st = admit ()
+
+let inverse_st_props (s:st{Seq.length (ops_of s) > 0})
+  : Lemma (let inv = inverse_st s in
+           init_of inv == init_of s /\
+           v_of s == do (v_of inv) (last (ops_of s)) /\
+           ops_of inv == Seq.slice (ops_of s) 0 (Seq.length (ops_of s) - 1))
+  = admit ()
+
 // length of both branches is > 0
-#set-options "--z3rlimit 1000"
+// #set-options "--z3rlimit 1000"
 let linearizable_ab_gt0 (lca a b:st)
   : Lemma
       (requires 
-          length (ops_of a) <> 0 /\ length (ops_of b) <> 0 /\
+          length (ops_of a) > 0 /\ length (ops_of b) > 0 /\
           v_of lca == init_of a /\
           init_of a == init_of b)
       (ensures 
          concrete_merge_pre (v_of lca) (v_of a) (v_of b) /\
          concrete_merge_pre (v_of lca) (inverse a) (inverse b) /\
          (let inv = concrete_merge (v_of lca) (inverse a) (inverse b) in
-            concrete_merge (v_of lca) (v_of a) (v_of b) =
-            seq_foldl do inv (resolve_conflict (last (ops_of a)) (last (ops_of b))) /\
-            (exists l. is_interleaving l (cons (last (ops_of a)) empty ) (cons (last (ops_of b)) empty) /\
-                  v_of (linearized_merge inv l) == concrete_merge (v_of lca) (v_of a) (v_of b))))
+          concrete_merge (v_of lca) (v_of a) (v_of b) =
+          seq_foldl do inv (resolve_conflict (last (ops_of a)) (last (ops_of b))) /\
+          (exists l. is_interleaving l (cons (last (ops_of a)) empty ) (cons (last (ops_of b)) empty) /\
+                v_of (linearized_merge inv l) == concrete_merge (v_of lca) (v_of a) (v_of b))))
   = lem_inverse a;
     lem_inverse b;
     assert (length (cons (last (ops_of a)) empty) = 1 /\ length (cons (last (ops_of b)) empty) = 1);
@@ -216,6 +255,7 @@ let linearizable_b_gt0 (lca a b:st)
 
 
 // length of both branches is 0
+#push-options "--z3rlimit 20"
 let linearizable_ab_0 (lca a b:st)
   : Lemma
       (requires 
@@ -227,27 +267,64 @@ let linearizable_ab_0 (lca a b:st)
          (exists l. is_interleaving l (ops_of a) (ops_of b) /\
                v_of (linearized_merge (v_of lca) l) == concrete_merge (v_of lca) (v_of a) (v_of b)))
   = assert (is_interleaving empty (ops_of a) (ops_of b)); ()
+#pop-options
 
+// #set-options "--initial_fuel 0 --max_fuel 2 --initial_ifuel 0 --max_ifuel 2 --z3rlimit 2000"
 
-#set-options "--initial_fuel 0 --max_fuel 2 --initial_ifuel 0 --max_ifuel 2 --z3rlimit 2000"
+let interleaving_predicate (l:log) (lca s1:st)
+  (s2:st{concrete_merge_pre (v_of lca) (v_of s1) (v_of s2)}) =
+  is_interleaving l (ops_of s1) (ops_of s2) /\
+  v_of (linearized_merge (v_of lca) l) ==
+  concrete_merge (v_of lca) (v_of s1) (v_of s2)
+
+#set-options "--z3rlimit 40 --fuel 2 --ifuel 2"
 let rec linearizable (lca s1 s2:st)
   : Lemma 
       (requires 
          v_of lca == init_of s1 /\
-         init_of s1 == init_of s2 (*)/\
-         distinct_ops (ops_of lca ++ (ops_of s1 ++ ops_of s2)*))
-      (ensures 
-         (exists l. is_interleaving l (ops_of s1) (ops_of s2) /\
+         init_of s1 == init_of s2)
+      (ensures
          concrete_merge_pre (v_of lca) (v_of s1) (v_of s2) /\
-         v_of (linearized_merge (v_of lca) l) == concrete_merge (v_of lca) (v_of s1) (v_of s2)))
+         (exists l. interleaving_predicate l lca s1 s2))
       (decreases %[length (ops_of s1); length (ops_of s2)])
 
-  = admit(); match length (ops_of s1), length (ops_of s2) with
-    |0,0 -> linearizable_ab_0 lca s1 s2
-    |0,_ -> linearizable_b_gt0 lca s1 s2
-    |_,0 -> linearizable_a_gt0 lca s1 s2
-    |_,_ -> linearizable_ab_gt0 lca s1 s2;
-           linearizable lca (seq_foldl do (init_of s1) (fst (un_snoc (ops_of s1))), 
-                             hide (init_of s1, (fst (un_snoc (ops_of s1)))))
-                            (seq_foldl do (init_of s2) (fst (un_snoc (ops_of s2))), 
-                             hide (init_of s2, (fst (un_snoc (ops_of s2)))))
+  = st_inv lca; st_inv s1; st_inv s2;
+    assert (concrete_merge_pre (v_of lca) (v_of s1) (v_of s2));
+    
+    if Seq.length (ops_of s1) = 0
+    then begin
+      linearized_merge_spec (v_of lca) (ops_of s2);
+      introduce exists l. interleaving_predicate l lca s1 s2
+      with (ops_of s2)
+      and ()
+    end
+    else begin
+      if Seq.length (ops_of s2) = 0
+      then begin
+        linearized_merge_spec (v_of lca) (ops_of s1);
+        introduce exists l. interleaving_predicate l lca s1 s2
+        with (ops_of s1)
+        and ()
+      end
+      else begin
+        let prefix1, hd1 = un_snoc (ops_of s1) in
+        let prefix2, hd2 = un_snoc (ops_of s2) in
+  
+        let inv1 = inverse_st s1 in
+        let inv2 = inverse_st s2 in
+
+        inverse_st_props s1;
+        inverse_st_props s2;
+
+        linearizable lca inv1 inv2;
+        eliminate exists l'. interleaving_predicate l' lca inv1 inv2
+        returns exists l. interleaving_predicate l lca s1 s2
+        with _. begin
+          let l = Seq.append l' (resolve_conflict hd1 hd2) in
+          introduce exists l. interleaving_predicate l lca s1 s2
+          with l
+          and interleaving_helper (ops_of s1) (ops_of s2) l';
+              admit ()
+        end
+      end
+    end
